Add local->public, fail trying to add unique->public

theories/tree_borrows/steps_opt.v
@@ -20,18 +20,252 @@ Implicit Types σ σ_s σ_t : state.
 Implicit Types r r_s r_t : result.
 Implicit Types l : loc.
 Implicit Types f : fname.
+
+Definition filter_unq_weak lp := match lp with 
+    Deallocable => Deallocable
+  | EnsuringAccess Strongly => EnsuringAccess Strongly
+  | EnsuringAccess WeaklyNoChildren => Deallocable end.
+(*
+TODO: this does not work because the invariant does not assert that no two calls can protect the same tag
+Lemma sim_make_unique_public l t ac (sc_s sc_t : list scalar) π Φ e_t e_s c M L:
+  l ↦t∗[tk_unq ac]{t} sc_t -∗
+  l ↦s∗[tk_unq ac]{t} sc_s -∗
+  t $$ tk_unq ac -∗
+  c @@ M ∗ ⌜M !! t = Some L ∧ L ≠ ∅⌝ -∗ (* TODO: L ≠ ∅ is required because things are, again set up per-offset sometimes but not always *)
+  value_rel sc_t sc_s -∗
+  (t $$ tk_pub -∗ c @@ <[t := fmap filter_unq_weak L]> M -∗ e_t ⪯{π} e_s [{ Φ }]) -∗
+  e_t ⪯{π} e_s [{ Φ }] .
+Proof.
+  iIntros "Ht Hs Htk (Hprot&%HL) #Hrel Hres".
+  iApply sim_update_si. rewrite /update_si. iIntros (?????) "(HP_t & HP_s & Hbor)".
+  iPoseProof (bor_interp_get_pure with "Hbor") as "%Hp".
+  destruct Hp as (Hsst_eq & Hstrs_eq & Hsnc_eq & Hscs_eq & Hwf_s & Hwf_t & Hdom_eq).
+  iDestruct "Hbor" as "(%M_call & %M_tag & %M_t & %M_s & Hbor)".
+  iDestruct "Hbor" as "((Hc & Htag_auth & Htag_t_auth & Htag_s_auth) & Hpub_cid & #Hsrel & %Hcall_interp & %Htag_interp & _)".
+  iPoseProof (tkmap_lookup with "Htag_auth Htk") as "%Ht_tk".
+  iAssert (|==> tkmap_auth tag_name 1 (<[ t := (tk_pub, ()) ]> M_tag) ∗ t $$ tk_pub)%I with "[Htag_auth Htk]" as ">(Htag_auth&Htk)".
+  { iMod (tkmap_update_strong tk_pub tt with "Htag_auth Htk") as "($&$)"; done. }
+  iPoseProof (ghost_map_lookup with "Htag_t_auth Ht") as "%Hhl_t".
+  iPoseProof (ghost_map_lookup with "Htag_s_auth Hs") as "%Hhl_s".
+  iMod (ghost_map_update ∅ with "Htag_t_auth Ht") as "(Htag_t_auth&_)".
+  iMod (ghost_map_update ∅ with "Htag_s_auth Hs") as "(Htag_s_auth&_)".
+  iPoseProof (ghost_map_lookup with "Hc Hprot") as "%Hprot".
+  iMod (ghost_map_update (<[t:=filter_unq_weak <$> L]> M) with "Hc Hprot") as "(Hc&Hprot)".
+  iAssert (⌜length sc_t = length sc_s⌝)%I as "%Hlen". 1: by iApply big_sepL2_length.
+
+  iModIntro. iSplitR "Hres Htk Hprot".
+  2: by iApply ("Hres" with "Htk Hprot").
+  iFrame "HP_s HP_t". iExists (<[c := _ ]> M_call), _, (<[(t, l.1):=∅]> M_t), (<[(t, l.1):=∅]> M_s).
+  iFrame "Hc Htag_t_auth Htag_s_auth Hpub_cid Htag_auth".
+  iSplit; last (iPureIntro; split; last (split; last done)).
+  - repeat (iSplit; first done). iDestruct "Hsrel" as "(_&_&_&_&_&Hsrel)".
+    iIntros (ll Hll). iDestruct ("Hsrel" $! ll Hll) as "[Hpub|(%tt&%Hpriv)]".
+    1: by iLeft.
+    destruct (decide (t = tt)) as [->|Hne].
+    2: { iRight. iPureIntro. exists tt.
+         rewrite /priv_loc lookup_insert_ne //.
+         rewrite /heaplet_lookup lookup_insert_ne //. 2: simpl; by congruence.
+         destruct Hpriv as (tk&H1&H2&H3). exists tk. split; first done. split; first done.
+         destruct H3 as [H3|(c'&ae'&H3A&H3B)]. 1: by left.
+         right. exists c', ae'. split; first done.
+         destruct H3B as (MM&HMM&H3B).
+         destruct (decide (c = c')) as [->|Hne'].
+         2: exists MM; split; last done; rewrite lookup_insert_ne //.
+         assert (M = MM) as -> by congruence.
+         eexists. rewrite lookup_insert. split; first done.
+         destruct H3B as (LL&HLL&H3B). exists LL.
+         rewrite lookup_insert_ne //. }
+    iLeft. rewrite /pub_loc. iIntros (sc_t' Hsc_t').
+    destruct Hpriv as (x&Htk'&Hheaplet&Hx). assert (x = tk_unq ac) as -> by congruence.
+    destruct Htag_interp as (Ht1&Ht2&Ht3&Ht4&Ht5).
+    destruct Hheaplet as (sc_ll&(hl_t'&Hheaplet_t1&Hheaplet_t2)%bind_Some).
+    simpl in Hheaplet_t1.
+    assert (l.1 = ll.1) as Hlleq.
+    { eapply Ht4. all: by eapply elem_of_dom_2. } rewrite /= -Hlleq Hhl_t in Hheaplet_t1.
+    injection Hheaplet_t1 as <-. simpl in Hheaplet_t2.
+    specialize (Ht1 _ _ Htk') as (HHt1&HHt2&HHt3&HHt4&HHt5).
+    ospecialize (HHt3 ll _ _).
+    1: rewrite /heaplet_lookup /= -Hlleq Hhl_t /= Hheaplet_t2 //.
+    assert (∃ sc_ll_s, list_to_heaplet sc_s l.2 !! ll.2 = Some sc_ll_s) as (sc_ll_s&Hsc_ll_s).
+    { eapply elem_of_dom. erewrite list_to_heaplet_dom_1. 2: symmetry; eapply Hlen. eapply elem_of_dom_2. eapply Hheaplet_t2. }
+    assert (∃ (i:nat), ll.2 = l.2 + i) as (i&Hoff).
+    { eapply list_to_heaplet_lookup_Some in Hsc_ll_s. exists (Z.to_nat (ll.2 - l.2)). lia. }
+    rewrite Hoff in Hsc_ll_s Hheaplet_t2.
+
+    destruct HHt3 as (_&HHt3).
+    { destruct Hx as [->|(c'&ae&->&Hcs)]. 1: done.
+      opose proof* (call_set_interp_access) as Hacc. 1: done. 1: exact Hcs.
+      destruct Hacc as (Hc&Hv&it&Hit&Hprot1&Hprot2&Hprot3&Hprot4).
+      exists it. split; first done. split; first done.
+      intros _ _. exists c'. split; done. }
+    specialize (HHt4 ll sc_ll_s).
+    destruct HHt4 as (_&HHt4).
+    1: rewrite /heaplet_lookup /= -Hlleq Hhl_s /= Hoff //.
+    { destruct Hx as [->|(c'&ae&->&Hcs)]. 1: done.
+      opose proof* (call_set_interp_access) as Hacc. 1: done. 1: exact Hcs.
+      destruct Hacc as (Hc&Hv&it&Hit&Hprot1&Hprot2&Hprot3&Hprot4).
+      odestruct trees_equal_find_equal_tag_protected_initialized_not_disabled as (it2&HH1&HH2&HH3).
+      1: by eapply trees_equal_sym. 2: exact Hprot4. 2: exists c'; by rewrite Hscs_eq.
+      1: done.
+      exists it2. split; first done. split; first done.
+      intros _ _. apply HH3. }
+    iExists sc_ll_s. iSplit; first done.
+    assert (sc_ll = sc_t') as <- by congruence.
+    rewrite !list_to_heaplet_nth in Hsc_ll_s Hheaplet_t2.
+    iPoseProof (big_sepL2_lookup_acc with "Hrel") as "($&_)".
+    all: done.
+  - intros c' M' [(<-&<-)|(Hne&HM')]%lookup_insert_Some.
+    + admit.
+    + specialize (Hcall_interp _ _ HM') as (H1&H2). split; first done.
+      intros tg' L' HL'. specialize (H2 _ _ HL') as (H2&H3). split; first done.
+      intros l' ps Hps. specialize (H3 _ _ Hps).
+      eapply tag_protected_for_mono. 2: exact H3.
+      intros [blk off] it Hlu Hiscall Hinit (tkp&Htag&Hheap).
+      exists tkp. Print call_set_interp. Print tag_protected_for.
+      assert (itag it ≠ t) as Hne2.
+      2: rewrite /heaplet_lookup !lookup_insert_ne /= //. 2: by intros [= ??].
+      intros <-.
+  - destruct Htag_interp as (H1&H2&H3&H4&H5). split_and!.
+    + intros tg tk' [(->&[= <-])|(Hne&Hin)]%lookup_insert_Some; last first.
+      * specialize (H1 _ _ Hin) as (HH1&HH2&HH3&HH4&HH5). split_and!.
+        1-2: done.
+        3: { rewrite /dom_agree_on_tag /heaplet_lookup /= //.
+             split; intros ?; rewrite !lookup_insert_ne; try congruence.
+             all: eapply HH5. }
+        { intros l' sc' H. rewrite /heaplet_lookup /= !lookup_insert_ne // in H. 2: congruence. 
+          by eapply HH3. }
+        { intros l' sc' H. rewrite /heaplet_lookup /= !lookup_insert_ne // in H. 2: congruence. 
+          by eapply HH4. }
+      * specialize (H1 _ _ Ht_tk) as (HH1&HH2&HH3&HH4&HH5). split_and!.
+        1-2: done.
+        3: { eapply dom_agree_on_tag_update_same. all: done. }
+        all: intros ??; rewrite /= /heaplet_lookup /=.
+        all: intros (x&[(?&<-)|(Hne&Hin)]%lookup_insert_Some&Hy)%bind_Some;
+          [rewrite lookup_empty // in Hy| ].
+        all: exfalso.
+        { ospecialize* H4. 1-2: eapply elem_of_dom_2. 1: exact Hin. 1: exact Hhl_t. congruence. }
+        { ospecialize* H5. 1-2: eapply elem_of_dom_2. 1: exact Hin. 1: exact Hhl_s. congruence. }
+    + intros t' blk H%elem_of_dom. rewrite dom_insert_lookup_L in H. 2: by eexists.
+      eapply elem_of_dom. rewrite dom_insert_lookup_L. 2: by eexists.
+      by eapply elem_of_dom, H2, elem_of_dom.
+    + intros t' blk H%elem_of_dom. rewrite dom_insert_lookup_L in H. 2: by eexists.
+      eapply elem_of_dom. rewrite dom_insert_lookup_L. 2: by eexists.
+      by eapply elem_of_dom, H3, elem_of_dom.
+    + intros tg blk1 blk2. rewrite !dom_insert_lookup_L. 2: by eexists.
+      by eapply H4.
+    + intros tg blk1 blk2. rewrite !dom_insert_lookup_L. 2: by eexists.
+      by eapply H5.
+Admitted.
+*)
+
+Lemma sim_make_local_public l t (sc_s sc_t : list scalar) π Φ e_t e_s:
+  l ↦t∗[tk_local]{t} sc_t -∗
+  l ↦s∗[tk_local]{t} sc_s -∗
+  t $$ tk_local -∗
+  value_rel sc_t sc_s -∗
+  (t $$ tk_pub -∗ e_t ⪯{π} e_s [{ Φ }]) -∗
+  e_t ⪯{π} e_s [{ Φ }] .
+Proof.
+  iIntros "Ht Hs Htk #Hrel Hres".
+  iApply sim_update_si. rewrite /update_si. iIntros (?????) "(HP_t & HP_s & Hbor)".
+  iPoseProof (bor_interp_get_pure with "Hbor") as "%Hp".
+  destruct Hp as (Hsst_eq & Hstrs_eq & Hsnc_eq & Hscs_eq & Hwf_s & Hwf_t & Hdom_eq).
+  iDestruct "Hbor" as "(%M_call & %M_tag & %M_t & %M_s & Hbor)".
+  iDestruct "Hbor" as "((Hc & Htag_auth & Htag_t_auth & Htag_s_auth) & Hpub_cid & #Hsrel & %Hcall_interp & %Htag_interp & _)".
+  iPoseProof (tkmap_lookup with "Htag_auth Htk") as "%Ht_tk".
+  iAssert (|==> tkmap_auth tag_name 1 (<[ t := (tk_pub, ()) ]> M_tag) ∗ t $$ tk_pub)%I with "[Htag_auth Htk]" as ">(Htag_auth&Htk)".
+  { iMod (tkmap_update_strong tk_pub tt with "Htag_auth Htk") as "($&$)"; done. }
+  iPoseProof (ghost_map_lookup with "Htag_t_auth Ht") as "%Hhl_t".
+  iPoseProof (ghost_map_lookup with "Htag_s_auth Hs") as "%Hhl_s".
+  iMod (ghost_map_update ∅ with "Htag_t_auth Ht") as "(Htag_t_auth&_)".
+  iMod (ghost_map_update ∅ with "Htag_s_auth Hs") as "(Htag_s_auth&_)".
+  iAssert (⌜length sc_t = length sc_s⌝)%I as "%Hlen". 1: by iApply big_sepL2_length.
+
+  iModIntro. iSplitR "Hres Htk".
+  2: by iApply "Hres".
+  iFrame "HP_s HP_t". iExists M_call, _, (<[(t, l.1):=∅]> M_t), (<[(t, l.1):=∅]> M_s).
+  iFrame "Hc Htag_t_auth Htag_s_auth Hpub_cid Htag_auth".
+  iSplit; last (iPureIntro; split; last (split; last done)).
+  - repeat (iSplit; first done). iDestruct "Hsrel" as "(_&_&_&_&_&Hsrel)".
+    iIntros (ll Hll). iDestruct ("Hsrel" $! ll Hll) as "[Hpub|(%tt&%Hpriv)]".
+    1: by iLeft.
+    destruct (decide (t = tt)) as [->|Hne].
+    2: { iRight. iPureIntro. exists tt.
+         rewrite /priv_loc lookup_insert_ne //.
+         rewrite /heaplet_lookup lookup_insert_ne //. simpl. by congruence. }
+    iLeft. rewrite /pub_loc. iIntros (sc_t' Hsc_t').
+    destruct Hpriv as (x&Htk'&Hheaplet&Hx). assert (x = tk_local) as -> by congruence.
+    destruct Htag_interp as (Ht1&Ht2&Ht3&Ht4&Ht5).
+    destruct Hheaplet as (sc_ll&(hl_t'&Hheaplet_t1&Hheaplet_t2)%bind_Some).
+    simpl in Hheaplet_t1.
+    assert (l.1 = ll.1) as Hlleq.
+    { eapply Ht4. all: by eapply elem_of_dom_2. } rewrite /= -Hlleq Hhl_t in Hheaplet_t1.
+    injection Hheaplet_t1 as <-. simpl in Hheaplet_t2.
+    specialize (Ht1 _ _ Htk') as (HHt1&HHt2&HHt3&HHt4&HHt5).
+    ospecialize (HHt3 ll _ _).
+    1: rewrite /heaplet_lookup /= -Hlleq Hhl_t /= Hheaplet_t2 //.
+    assert (∃ sc_ll_s, list_to_heaplet sc_s l.2 !! ll.2 = Some sc_ll_s) as (sc_ll_s&Hsc_ll_s).
+    { eapply elem_of_dom. erewrite list_to_heaplet_dom_1. 2: symmetry; eapply Hlen. eapply elem_of_dom_2. eapply Hheaplet_t2. }
+    assert (∃ (i:nat), ll.2 = l.2 + i) as (i&Hoff).
+    { eapply list_to_heaplet_lookup_Some in Hsc_ll_s. exists (Z.to_nat (ll.2 - l.2)). lia. }
+    rewrite Hoff in Hsc_ll_s Hheaplet_t2.
+
+    destruct HHt3 as (_&HHt3).
+    { destruct Hx as [|(c&ae&Heq&Hcs)]. 1: done. exfalso. congruence. }
+    specialize (HHt4 ll sc_ll_s).
+    destruct HHt4 as (_&HHt4).
+    1: rewrite /heaplet_lookup /= -Hlleq Hhl_s /= Hoff //.
+    { destruct Hx as [|(c&ae&Heq&Hcs)]. 1: done. exfalso. congruence. }
+    iExists sc_ll_s. iSplit; first done.
+    assert (sc_ll = sc_t') as <- by congruence.
+    rewrite !list_to_heaplet_nth in Hsc_ll_s Hheaplet_t2.
+    iPoseProof (big_sepL2_lookup_acc with "Hrel") as "($&_)".
+    all: done.
+  - intros c M' HM'. specialize (Hcall_interp _ _ HM') as (H1&H2). split; first done.
+    intros tg' L HL. specialize (H2 _ _ HL) as (H2&H3). split; first done.
+    intros l' ps Hps. specialize (H3 _ _ Hps).
+    eapply tag_protected_for_mono. 2: exact H3.
+    intros [blk off] it Hlu Hiscall Hinit (tkp&Htag&Hheap).
+    exists tkp. assert (itag it ≠ t) as Hne.
+    { intros <-. congruence. }
+    rewrite lookup_insert_ne //. split; first done.
+    rewrite /heaplet_lookup lookup_insert_ne /= //.
+    intros [= ??]; done.
+  - destruct Htag_interp as (H1&H2&H3&H4&H5). split_and!.
+    + intros tg tk' [(->&[= <-])|(Hne&Hin)]%lookup_insert_Some; last first.
+      * specialize (H1 _ _ Hin) as (HH1&HH2&HH3&HH4&HH5). split_and!.
+        1-2: done.
+        3: { rewrite /dom_agree_on_tag /heaplet_lookup /= //.
+             split; intros ?; rewrite !lookup_insert_ne; try congruence.
+             all: eapply HH5. }
+        { intros l' sc' H. rewrite /heaplet_lookup /= !lookup_insert_ne // in H. 2: congruence. 
+          by eapply HH3. }
+        { intros l' sc' H. rewrite /heaplet_lookup /= !lookup_insert_ne // in H. 2: congruence. 
+          by eapply HH4. }
+      * specialize (H1 _ _ Ht_tk) as (HH1&HH2&HH3&HH4&HH5). split_and!.
+        1-2: done.
+        3: { eapply dom_agree_on_tag_update_same. all: done. }
+        all: intros ??; rewrite /= /heaplet_lookup /=.
+        all: intros (x&[(?&<-)|(Hne&Hin)]%lookup_insert_Some&Hy)%bind_Some;
+          [rewrite lookup_empty // in Hy| ].
+        all: exfalso.
+        { ospecialize* H4. 1-2: eapply elem_of_dom_2. 1: exact Hin. 1: exact Hhl_t. congruence. }
+        { ospecialize* H5. 1-2: eapply elem_of_dom_2. 1: exact Hin. 1: exact Hhl_s. congruence. }
+    + intros t' blk H%elem_of_dom. rewrite dom_insert_lookup_L in H. 2: by eexists.
+      eapply elem_of_dom. rewrite dom_insert_lookup_L. 2: by eexists.
+      by eapply elem_of_dom, H2, elem_of_dom.
+    + intros t' blk H%elem_of_dom. rewrite dom_insert_lookup_L in H. 2: by eexists.
+      eapply elem_of_dom. rewrite dom_insert_lookup_L. 2: by eexists.
+      by eapply elem_of_dom, H3, elem_of_dom.
+    + intros tg blk1 blk2. rewrite !dom_insert_lookup_L. 2: by eexists.
+      by eapply H4.
+    + intros tg blk1 blk2. rewrite !dom_insert_lookup_L. 2: by eexists.
+      by eapply H5.
+Qed.
+  
+
 (*
 
-Lemma sim_protected_unprotect M L l c t tk sc_t sc_s π Φ e_t e_s :
-  l ∈ L →
-  M !! t = Some L →
-  c @@ M -∗
-  t $$ tk -∗
-  l ↦t[tk]{t} sc_t -∗
-  l ↦s[tk]{t} sc_s -∗
-  sc_rel sc_t sc_s -∗
-  (c @@ (<[t := L ∖ {[ l ]} ]> M) -∗ t $$ tk -∗ l ↦t[tk]{t} sc_t -∗ l ↦s[tk]{t} sc_s -∗ e_t ⪯{π} e_s [{ Φ }]) -∗
-  e_t ⪯{π} e_s [{ Φ }].
 Proof.
   iIntros (Hin HL) "Hc Htag Ht Hs Hrel Hsim".
   iApply (sim_protected_unprotectN M L l c t tk [sc_t] [sc_s] with "Hc Htag [Ht] [Hs] [Hrel] [Hsim]").
